theories/PiggyBank.v
@@ -1,0 +1,244 @@
+From stdpp Require Import namespaces.
+From iris.base_logic.lib Require Import na_invariants.
+From iris_time.heap_lang Require Import proofmode notation.
+From iris_time Require Import TimeCredits Auth_max_nat.
+
+(* -------------------------------------------------------------------------- *)
+
+Section PiggyBank.
+
+Context `{timeCreditHeapG Σ}.
+Context `{inG Σ (authR max_natUR)}.                   (* γpaid *)
+Context `{na_invG Σ}.
+Notation iProp := (iProp Σ).
+
+Implicit Type p : na_inv_pool_name.
+Implicit Type N : namespace.
+Implicit Type n nc ac : nat.
+Implicit Type R : iProp.
+Implicit Type φ : val → iProp.
+Implicit Type γpaid : gname.
+
+Variable LeftBranch  : (* nc: *) nat → iProp.
+Variable RightBranch : (* nc: *) nat → iProp.
+
+Definition PiggyBankInvariant γpaid nc : iProp :=
+  ∃ ac,
+      own γpaid (● MaxNat ac)
+    ∗ ((LeftBranch nc ∗ TC ac) ∨ (RightBranch nc ∗ ⌜ nc ≤ ac ⌝)).
+
+Definition PiggyBank p N n : iProp :=
+  ∃ γpaid nc,
+      na_inv p N (PiggyBankInvariant γpaid nc)
+    ∗ own γpaid (◯ MaxNat (nc - n)).
+
+(* -------------------------------------------------------------------------- *)
+
+(* Local tactics, for clarity. *)
+
+Local Ltac destruct_piggy :=
+  iDestruct "Hpiggy" as (γpaid nc) "(Hinv & Hγpaid◯)".
+
+Local Ltac open_invariant :=
+  iDestruct (na_inv_acc with "Hinv Htoken") as ">(Hbank & Htoken & Hclose)";
+    [set_solver | set_solver |];
+  iDestruct "Hbank" as (ac) "(>Hγpaid● & Hbank)".
+
+Local Ltac case_analysis :=
+  iDestruct "Hbank" as "[ (Hbranch & >Hac) | (Hbranch & >%Hncac) ]".
+
+Local Ltac create_white_bullet :=
+  iMod (auth_max_nat_update_read_auth with "Hγpaid●")
+    as "(Hγpaid● & #Hγpaid◯)".
+
+Local Ltac weaken_white_bullet :=
+  iDestruct (own_auth_max_nat_weaken with "Hγpaid◯") as "$";
+  lia.
+
+Local Ltac exploit_white_bullet :=
+  iDestruct (own_auth_max_nat_le with "Hγpaid● Hγpaid◯") as "%Hleq".
+
+Local Ltac increase_black_bullet k :=
+  iMod (auth_max_nat_update_incr _ _ k with "Hγpaid●") as "Hγpaid●".
+
+Local Ltac close_invariant ac :=
+  iMod ("Hclose" with "[-]") as "$"; [
+    (* Subgoal: prove that the invariant holds *)
+    iFrame "Htoken"; iNext; iExists ac; iFrame "Hγpaid●"
+  | (* Subgoal: after the invariant is closed *)
+    iModIntro (* We assume that we do not need the modality any more. *)
+  ].
+
+Local Ltac construct_piggy :=
+  iExists _, _; iFrame "Hinv"; weaken_white_bullet.
+
+(* -------------------------------------------------------------------------- *)
+
+(* Properties. *)
+
+Global Instance piggybank_persistent p N n :
+  Persistent (PiggyBank p N n).
+Proof using.
+  exact _.
+Qed.
+
+Lemma piggybank_discover_zero_debit p N n E F :
+  ↑N ⊆ E →
+  ↑N ⊆ F →
+  PiggyBank p N n -∗
+  na_own p F -∗
+  (∀ nc, ▷ LeftBranch nc -∗ ▷ False) ={E}=∗
+  PiggyBank p N 0 ∗
+  na_own p F.
+Proof.
+  intros.
+  iIntros "#Hpiggy Htoken Hcontradiction".
+  destruct_piggy.
+  open_invariant.
+  case_analysis.
+
+  (* Case: left branch. This is impossible. *)
+  { iDestruct ("Hcontradiction" with "Hbranch") as ">contradiction".
+      (* Because the goal is an update, we can strip a ▷ modality. *)
+    iExFalso. eauto. }
+
+  (* Case: right branch. *)
+  iClear "Hcontradiction".
+  iClear "Hγpaid◯".
+  (* We have [nc ≤ ac]. We may create a ghost witness of this fact.
+     This will allow us to argue that this piggy bank has debt zero. *)
+  create_white_bullet.
+  (* Close the invariant. *)
+  close_invariant ac.
+  { iRight. eauto. }
+  construct_piggy.
+
+Qed.
+
+Lemma piggy_bank_increase_debt p N n1 n2 :
+  n1 ≤ n2 →
+  PiggyBank p N n1 -∗
+  PiggyBank p N n2.
+Proof.
+  intros.
+  iIntros "#Hpiggy".
+  destruct_piggy.
+  construct_piggy.
+Qed.
+
+Lemma piggybank_create p N nc E :
+  TC 0 -∗
+  LeftBranch nc ={E}=∗
+  PiggyBank p N nc.
+Proof.
+  iIntros "Htc Hleft".
+  (* Allocate the ghost cell γpaid. *)
+  iMod (auth_max_nat_alloc 0) as (γpaid) "[Hγpaid● #Hγpaid◯]".
+  (* Allocate an invariant. The number of credits in the bank is zero. *)
+  iAssert (PiggyBankInvariant γpaid nc) with "[-]" as "Hbank".
+  { iExists 0. iFrame "Hγpaid●". iLeft. eauto. }
+  iMod (na_inv_alloc with "Hbank") as "Hinv";
+  iModIntro.
+  construct_piggy.
+Qed.
+
+Lemma piggybank_break p N E F :
+  let token := na_own p F in
+  let token' := na_own p (F ∖ ↑N) in
+  ↑N ⊆ E →
+  ↑N ⊆ F →
+  PiggyBank p N 0 -∗
+  token
+   ={E}=∗
+   ( ∃ nc,
+      ▷ LeftBranch nc ∗ TC nc ∗ token' ∗
+     (▷ RightBranch nc -∗ token' ={E}=∗ token)
+   ) ∨
+   ( ∃ nc,
+      ▷ RightBranch nc ∗ token' ∗
+     (▷ RightBranch nc -∗ token' ={E}=∗ token)
+   ).
+Proof.
+  intros.
+  iIntros "#Hpiggy Htoken".
+  destruct_piggy.
+  rewrite Nat.sub_0_r.
+  open_invariant.
+  case_analysis;
+  iModIntro.
+
+  (* Case: left branch. *)
+  {
+    (* We are in the left-hand branch of the conclusion. *)
+    iLeft. iExists nc. iFrame "Hbranch Htoken".
+    (* The number of debits is zero, so we learn [nc ≤ ac]. *)
+    exploit_white_bullet.
+    (* Therefore, we have the necessary time credits at hand. *)
+    iDestruct (TC_weaken _ _ Hleq with "Hac") as "$".
+    (* Once the user performs a state change to [RightBranch nc],
+       we will be able to close the invariant. *)
+    iIntros "Hbranch Htoken".
+    close_invariant ac; [| done ].
+    { iRight. eauto. }
+  }
+
+  (* Case: right branch. This case is trivial. *)
+  {
+    (* We are in the right-hand branch of the conclusion. *)
+    iRight. iExists nc. iFrame "Hbranch Htoken".
+    (* Once the user performs a state change to [RightBranch nc],
+       we will be able to close the invariant. *)
+    iIntros "Hbranch Htoken".
+    close_invariant ac; [| done ].
+    { iRight. eauto. }
+  }
+
+Qed.
+
+Lemma piggybank_pay k p N E F n :
+  ↑N ⊆ E →
+  ↑N ⊆ F →
+  na_own p F -∗ PiggyBank p N n -∗   TC k   ={E}=∗
+  na_own p F  ∗ PiggyBank p N (n-k).
+Proof.
+  intros.
+  iIntros "Htoken #Hpiggy Hk".
+  destruct_piggy.
+  open_invariant.
+
+  (* We learn [nc - n ≤ ac]. *)
+  exploit_white_bullet.
+
+  (* Increment the ghost payment record from [ac] to [ac + k]. *)
+  increase_black_bullet k.
+  iClear "Hγpaid◯".
+  create_white_bullet.
+
+  (* Perform a case analysis. *)
+  case_analysis.
+
+  (* Case: left branch. *)
+  {
+    (* We have [ac + k] time credits. *)
+    iCombine "Hac Hk" as "Hac".
+    (* The invariant can be closed. *)
+    close_invariant (ac + k).
+    { iLeft. eauto with iFrame. }
+    (* Our updated fragmentary view of the ghost cell γpaid
+       allows us to produce an updated [PiggyBank] assertion. *)
+    construct_piggy.
+  }
+
+  (* Case: right branch. *)
+  {
+    (* The invariant can be closed. In this case, no new time credits are
+       stored in the invariant. The extra payment is wasted. *)
+    iClear "Hk".
+    close_invariant (ac + k).
+    { iRight. eauto with lia iFrame. }
+    construct_piggy.
+  }
+
+Qed.
+
+End PiggyBank.
